src/goose_lang/lib/string/string.v
@@ -6,62 +6,154 @@ Section heap.
 Context `{ffi_sem: ffi_semantics} `{!ffi_interp ffi} `{!heapGS Σ}.
 Context {ext_ty: ext_types ext}.
 
-Fixpoint string_to_bytes (s:string): list u8 :=
-  match s with
-  | EmptyString => []
-  | String x srest => [U8 (Ascii.nat_of_ascii x)] ++ (string_to_bytes srest)
-  end
-.
+Definition string_to_bytes (s:string): list u8 :=
+  (λ x, U8 $ Ascii.nat_of_ascii x) <$> list_ascii_of_string s.
 
 Definition bytes_to_string (l:list u8) : string :=
-  fold_right (λ b s, (u8_to_string b) +:+ s) EmptyString l
-.
+  string_of_list_ascii (u8_to_ascii <$> l).
+
+(*
+Ltac word_cleanup :=
+  repeat autounfold with word in *;
+  try match goal with
+      | |- @eq u64 _ _ => apply word.unsigned_inj
+      | |- @eq u32 _ _ => apply word.unsigned_inj
+      | |- @eq u8 _ _ => apply word.unsigned_inj
+      end;
+  (* can't replace this with [autorewrite], probably because typeclass inference
+  isn't the same *)
+  rewrite ?word.unsigned_add, ?word.unsigned_sub,
+  ?word.unsigned_divu_nowrap, ?word.unsigned_modu_nowrap,
+  ?unsigned_U64_0, ?unsigned_U32_0,
+  ?word.unsigned_of_Z, ?word.of_Z_unsigned, ?unsigned_U64, ?unsigned_U32;
+  try autorewrite with word;
+  repeat match goal with
+         | [ H: context[word.unsigned (U64 (Zpos ?x))] |- _ ] => change (int.Z (Zpos x)) with (Zpos x) in *
+         | [ |- context[word.unsigned (U64 (Zpos ?x))] ] => change (int.Z (Zpos x)) with (Zpos x)
+         | [ H: context[word.unsigned (U32 (Zpos ?x))] |- _ ] => change (int.Z (U32 (Zpos x))) with (Zpos x) in *
+         | [ |- context[word.unsigned (U32 (Zpos ?x))] ] => change (int.Z (U32 (Zpos x))) with (Zpos x)
+         end;
+  repeat match goal with
+         | [ |- context[int.Z ?x] ] =>
+           lazymatch goal with
+           | [ H': 0 <= int.Z x < 2^64 |- _ ] => fail
+           | [ H': 0 <= int.Z x <= 2^64 |- _ ] => fail (* TODO: should be unnecessary *)
+           | _ => pose proof (word.unsigned_range x)
+           end
+         | [ H: context[int.Z ?x] |- _ ] =>
+           lazymatch goal with
+           | [ H': 0 <= int.Z x < 2^64 |- _ ] => fail
+           | [ H': 0 <= int.Z x <= 2^64 |- _ ] => fail (* TODO: should be unnecessary *)
+           | _ => pose proof (word.unsigned_range x)
+           end
+         end;
+  repeat match goal with
+         | |- context[@word.wrap _ ?word ?ok ?z] =>
+           rewrite (@wrap_small _ word ok z) by lia
+         | |- context[Z.of_nat (Z.to_nat ?z)] =>
+           rewrite (Z2Nat.id z) by lia
+         end;
+  try lia. *)
 
 Lemma byte_to_string_inj l :
   string_to_bytes $ bytes_to_string l = l.
 Proof.
-  induction l as [|].
-  { done. }
+  rewrite /string_to_bytes /bytes_to_string /=.
+  rewrite -{2}(list_fmap_id l).
+  rewrite list_ascii_of_string_of_list_ascii.
+  rewrite -list_fmap_compose.
+  apply list_fmap_ext.
+  intros.
+  simpl.
+  rewrite /string_to_bytes /bytes_to_string /= /u8_to_ascii.
+  pose proof (word.unsigned_range x).
+  assert (int.nat x < 256)%nat.
+  { lia. (* word_cleanup. *) } (* FIXME: word_cleanup doesn't have good support for u8  *)
+  rewrite Ascii.nat_ascii_embedding.
   {
-    rewrite /string_to_bytes /bytes_to_string /= /u8_to_ascii.
-    assert (int.nat a < 256)%nat.
-    { clear -a. admit. } (* FIXME: word (same as above) *)
-    rewrite Ascii.nat_ascii_embedding.
-    {
-      f_equal.
-      { clear -a. admit. } (* FIXME: word *)
-      done.
-    }
-    { done. }
+    apply word.unsigned_inj.
+    rewrite (Z2Nat.id _); last lia.
+    rewrite word.unsigned_of_Z.
+    by rewrite (@wrap_small _ _ _ _).
   }
-Admitted.
+  done.
+Qed.
 
 Lemma string_to_bytes_app s1 s2 :
   string_to_bytes (s1 ++ s2) = string_to_bytes s1 ++ string_to_bytes s2.
 Proof.
+  rewrite /string_to_bytes.
 Admitted.
 
 Lemma string_to_bytes_inj s :
    bytes_to_string $ string_to_bytes s = s.
 Proof.
+  rewrite /string_to_bytes /bytes_to_string /=.
   induction s as [|].
   { done. }
   {
-    replace (String a s) with ((String a EmptyString) +:+ s) by done.
-    rewrite string_to_bytes_app.
     simpl.
     rewrite IHs.
     f_equal.
     rewrite /u8_to_string /u8_to_ascii.
     f_equal.
     replace (int.nat (_)) with (Ascii.nat_of_ascii a).
-    2:{ Search Ascii.nat_of_ascii.
-        pose proof (Ascii.nat_ascii_bounded a) as H.
+    2:{ pose proof (Ascii.nat_ascii_bounded a) as H.
         revert H. generalize (Ascii.nat_of_ascii a).
-        intros. admit. (* FIXME: word. *)
+        intros.
+        rewrite word.unsigned_of_Z.
+        word.
     }
     by rewrite Ascii.ascii_nat_embedding.
   }
+Qed.
+
+(*
+Global Instance pure_StringGet s i c :
+  PureExec (bin_op_eval op v1 v2 = Some c) 1 (BinOp StringGetOp (Val $ LitString $ s)
+                                                     (Val $ LitInt $ i)) (c) | 10.
+Proof. solve_pure_exec. Qed. *)
+
+Lemma wp_stringToBytes (i:u64) (s:string) :
+  {{{
+        ⌜int.nat i <= String.length s⌝
+  }}}
+    stringToBytes #i #(str s)
+  {{{
+        (sl:Slice.t), RET (slice_val sl); own_slice sl byteT 1
+                                                    (take (int.nat i) (string_to_bytes s))
+  }}}
+.
+Proof.
+  iLöb as "Hwp" forall (i).
+  iIntros (Φ) "%Hineq HΦ".
+  wp_rec.
+  wp_pures.
+  wp_if_destruct.
+  {
+    change (slice.nil) with (slice_val Slice.nil).
+    iApply "HΦ". iModIntro.
+    rewrite take_0.
+    by iApply (own_slice_nil).
+  }
+  wp_pures.
+  wp_pure1.
+  { (* FIXME: StringGet wp_pures *)
+    rewrite /bin_op_eval /=.
+    instantiate (1:=(LitV $ LitByte $ (U8 37))).
+    admit.
+  }
+  wp_pures.
+  wp_apply ("Hwp" with "[]").
+  {
+    iPureIntro. admit. (* TODO: overflow reasoning *)
+  }
+  iIntros (?) "Hsl'".
+  change (#(U8 37)) with (into_val.to_val (U8 37)).
+  wp_apply (wp_SliceAppend with "[$]").
+  iIntros (?) "Hsl".
+  iApply "HΦ".
+  (* FIXME: appending in wrong order *)
 Admitted.
 
 Lemma wp_StringToBytes (s:string) :
@@ -74,6 +166,14 @@ Lemma wp_StringToBytes (s:string) :
   }}}
 .
 Proof.
+  iIntros (Φ) "Hsl HΦ".
+  wp_lam. wp_pures.
+  wp_apply wp_stringToBytes.
+  { admit. (* TODO: overflow *) }
+  iIntros. iApply "HΦ".
+  rewrite take_ge.
+  { iFrame. }
+  admit. (* TODO: overflow and length of string_to_bytes vs String.length *)
 Admitted.
 
 Lemma wp_StringFromBytes sl q (l:list u8) :
