external/Goose/github_com/tchajed/goose/internal/examples/semantics.v
@@ -1144,7 +1144,6 @@ Definition stringLength: val :=
   rec: "stringLength" "s" :=
     StringLength "s".
 
-(* tests *)
 Definition failing_testStringAppend: val :=
   rec: "failing_testStringAppend" <> :=
     let: "ok" := ref_to boolT #true in
