src/goose_lang/notation.v
@@ -105,6 +105,7 @@ Notation "'to_u8' e" := (UnOp ToUInt8Op e%E) (at level 10) : expr_scope.
 Notation "'to_string' e" := (UnOp ToStringOp e%E) (at level 10) : expr_scope.
 Notation "'StringLength' e" := (UnOp StringLenOp e%E) (at level 10) : expr_scope.
 
+Notation "'StringGet'" := (BinOp StringGetOp) (at level 10) : expr_scope.
 Notation "e1 + e2" := (BinOp PlusOp e1%E e2%E) : expr_scope.
 Notation "e1 +ₗ e2" := (BinOp (OffsetOp 1) e1%E e2%E) : expr_scope.
 Notation "e1 - e2" := (BinOp MinusOp e1%E e2%E) : expr_scope.
